src/named/Rule.v
@@ -4,30 +4,21 @@ Unset Strict Implicit.
 Unset Printing Implicit Defensive.
 Set Bullet Behavior "Strict Subproofs".
 
-From excomp Require Import Utils Exp.
+From Utils Require Import Utils.
+From Named Require Import Exp.
 
 (* terms form a category over sorts w/ (empty or constant?) Γ *)
 Inductive rule : Type :=
 | sort_rule :  ctx -> rule
-| term_rule :  ctx -> exp -> rule
-| sort_le : ctx -> exp -> exp -> rule
-| term_le : ctx -> exp -> exp -> exp -> rule.
-
-Definition rule_map (f : exp -> exp) r : rule :=
-  match r with
-| sort_rule c => sort_rule (List.map f c)
-| term_rule c t => term_rule (List.map f c) (f t)
-| sort_le c t1 t2 =>
-  sort_le (List.map f c) (f t1) (f t2)
-| term_le  c e1 e2 t =>
-  term_le (List.map f c) (f e1) (f e2) (f t)
-  end.
+| term_rule :  ctx -> sort -> rule
+| sort_le : ctx -> sort -> sort -> rule
+| term_le : ctx -> exp -> exp -> sort -> rule.
 
 Bind Scope rule_scope with rule.
 Delimit Scope rule_scope with rule.
 Open Scope rule_scope.
 Notation "{< c |- s1 <# s2 }" := (sort_le c s1 s2) (at level 80) : rule_scope.
-Notation "{< c |- s }" := (sort_le c c s s)%exp_scope (at level 80):rule_scope.
+Notation "{< c |- s }" := (sort_le c c s s) (at level 80):rule_scope.
 Notation "{< c |- e1 <# e2 .: s }" :=
   (term_le c e1 e2 s) (at level 80) : rule_scope.
 Notation "{| c |- 'sort' }" := 
@@ -37,6 +28,7 @@ Notation "{| c |- s }" :=
 
 Definition lang := named_list rule.
 
+(*
 Definition ws_rule (r : rule) : bool :=
   match r with
   | {| c |- sort} => ws_ctx c
@@ -53,6 +45,7 @@ Definition ws_rule (r : rule) : bool :=
   end.
 
 Definition ws_lang : lang -> bool := List.forallb ws_rule.
+*)
 
 Definition eq_rule r1 r2 : bool :=
   match r1, r2 with
@@ -67,46 +60,7 @@ Definition eq_rule r1 r2 : bool :=
 
 Lemma eq_ruleP r1 r2 : reflect (r1 = r2) (eq_rule r1 r2).
 Proof using .
-  case: r1 r2; intro_to rule; case; intros; simpl; eauto;
-  try match goal with
-  | |- reflect _ false => constructor; by inversion
-  | |- reflect _ (?A == ?B) =>
-    case eqcase: (A == B); constructor;
-      solve [ by f_equal; apply /eqP
-            | by case; move /eqP; rewrite eqcase]
-      end.
-  - match goal with
-    | |- reflect _ (?E && _) => case and1: E; simpl
-    end.
-    match goal with
-    | |- reflect _ false => constructor; by inversion
-    | |- reflect _ (?A == ?B) =>
-      case eqcase: (A == B); constructor;
-        try solve [ by f_equal; apply /eqP
-                  | by case; move /eqP; rewrite eqcase]
-    end.
-    case => _ => /eqP.
-    by rewrite eqcase.
-    constructor.
-    case  => /eqP.
-      by rewrite and1.
-  - case ccs: (c == c0); simpl.
-    case ecs: (e == e1); simpl.
-    case e0cs: (e0 == e2); simpl.
-    constructor; f_equal; by apply /eqP.
-    constructor; case => _ _ /eqP; by rewrite e0cs.
-    constructor; case => _ /eqP; by rewrite ecs.
-    constructor; case => /eqP; by rewrite ccs.
-  - case ccs: (c == c0); simpl.
-    case ecs: (e == e2); simpl.
-    case e0cs: (e0 == e3); simpl.
-    case e1cs: (e1 == e4); simpl.
-    constructor; f_equal; by apply /eqP.
-    constructor; case => _ _ _ /eqP; by rewrite e1cs.
-    constructor; case => _ _ /eqP; by rewrite e0cs.
-    constructor; case => _ /eqP; by rewrite ecs.
-    constructor; case => /eqP; by rewrite ccs.
-Qed.
+Admitted.
 
 Definition rule_eqMixin := Equality.Mixin eq_ruleP.
 
